cfrontend/Cminorgenproof.v
@@ -36,11 +36,13 @@ Section TRANSLATION.
 Variable prog: Csharpminor.program.
 Variable tprog: program.
 Hypothesis TRANSL: match_prog prog tprog.
-Variable w: meminj.
+Variable w: meminj_thr.
 Variable se: Genv.symtbl.
 Variable tse: Genv.symtbl.
 Let ge : Csharpminor.genv := Genv.globalenv se prog.
 Let tge: genv := Genv.globalenv tse tprog.
+
+Hypothesis GE: cc_inj_senv w se tse.
 
 Lemma functions_translated (j: meminj):
   Genv.match_stbls j se tse ->
@@ -438,8 +440,7 @@ Inductive match_callstack (f: meminj) (m: mem) (tm: mem):
                           callstack -> block -> block -> Prop :=
   | mcs_nil:
       forall bound tbound,
-      inject_incr w f ->
-      Genv.match_stbls f se tse ->
+      mit_incr w f ->
       Ple (Genv.genv_next ge) bound -> Ple (Genv.genv_next tge) tbound ->
       match_callstack f m tm nil bound tbound
   | mcs_cons:
@@ -461,6 +462,7 @@ Lemma match_callstack_match_globalenvs:
   Genv.match_stbls f se tse.
 Proof.
   induction 1; eauto.
+  eapply cc_inj_match_stbls; eauto.
 Qed.
 
 (** Invariance properties for [match_callstack]. *)
@@ -478,9 +480,12 @@ Proof.
   induction 1; intros.
   (* base case *)
   econstructor; eauto.
-  eapply inject_incr_trans; eauto.
-  eapply Genv.match_stbls_incr; eauto.
-  intros. eapply H7; eauto. eapply Pos.lt_le_trans; eauto.
+  destruct H as [Hf1 SEP]. split; eauto using inject_incr_trans.
+  inv GE. cbn in *. intros. destruct (f1 b1) as [[xb2 xdelta] | ] eqn:Hb1.
+    eapply SEP; eauto. rewrite Hb1. apply H2 in Hb1. rewrite <- Hb1. eauto.
+    destruct (plt b1 bound). rewrite H5 in H8; eauto.
+    destruct (plt b2 tbound). erewrite H6 in Hb1; eauto.
+    xomega.
   (* inductive case *)
   assert (Ple lo hi) by (eapply me_low_high; eauto).
   econstructor; eauto.
@@ -601,12 +606,11 @@ Proof.
   induction 1; intros.
 (* base case *)
   apply mcs_nil; auto.
-  eapply inject_incr_trans; eauto.
-  eapply Genv.match_stbls_incr; eauto.
+  destruct H as [H SEP]. split. eapply inject_incr_trans; eauto.
   intros. case_eq (f1 b1).
   intros [b2' delta'] EQ. rewrite (INCR _ _ _ EQ) in H5. inv H5. eauto.
-  intro EQ. exploit SEPARATED; eauto. intros [A B]. elim B. red.
-  apply Mem.unchanged_on_nextblock in OUTOFREACH. eapply Pos.lt_le_trans, Pos.le_trans; eauto.
+  intro EQ. exploit SEPARATED; eauto. intros [A B].
+  unfold Mem.valid_block in *. inv GE; cbn in *. xomega.
 (* inductive case *)
   constructor. auto. auto.
   eapply match_temps_invariant; eauto.
@@ -2158,17 +2162,17 @@ Opaque PTree.set.
 Qed.
 
 Lemma transl_initial_states:
-  forall q1 q2, Genv.match_stbls w se tse -> cc_inj_query w q1 q2 ->
+  forall q1 q2, cc_inj_query w q1 q2 ->
   forall S, Csharpminor.initial_state ge q1 S ->
   exists R, Cminor.initial_state tge q2 R /\ match_states S R.
 Proof.
-  intros _ _ Hse [vf1 vf2 sg vargs1 vargs2 m1 m2 Hvf Hvargs Hm] S HS. inv HS.
-  exploit functions_translated; eauto. intros [tf [FIND TR]].
+  intros _ _ [vf1 vf2 sg vargs1 vargs2 m1 m2 Hvf Hvargs Hm] S HS. inv HS.
+  exploit functions_translated; eauto. destruct GE; auto. intros [tf [FIND TR]].
   setoid_rewrite <- (sig_preserved _ _ TR). monadInv TR. cbn.
   econstructor; split.
   econstructor; eauto.
   eapply match_callstate with (f := w) (cs := @nil frame) (cenv := PTree.empty Z); auto.
-  apply mcs_nil; auto. admit. admit. (* nextblock *)
+  apply mcs_nil; auto using mit_incr_refl. admit. admit. (* nextblock *)
   constructor. red; auto.
 Admitted.
 
@@ -2178,24 +2182,29 @@ Lemma transl_final_states:
 Proof.
   intros. inv H0. inv H. inv MK. inv MCS.
   eexists; split. constructor. econstructor; eauto.
+  inv GE; cbn in *; eauto.
+  inv GE; cbn in *; eauto.
 Qed.
 
 Lemma transl_external_states:
   forall S R q1, match_states S R -> Csharpminor.at_external ge S q1 ->
-  exists wx q2, Cminor.at_external tge R q2 /\ cc_injp_query wx q1 q2 /\ Genv.match_stbls wx se tse /\
+  exists wx q2, Cminor.at_external tge R q2 /\ cc_injp_query wx q1 q2 /\ cc_injp_stbls wx se tse /\
   forall r1 r2 S', cc_injp_reply wx r1 r2 -> Csharpminor.after_external S r1 S' ->
   exists R', Cminor.after_external R r2 R' /\ match_states S' R'.
 Proof.
   intros S R q1 HSR Hq1.
   destruct Hq1; inv HSR.
+  assert (vf <> Vundef) by (intro; subst; discriminate).
   eapply functions_translated in H as (tfd & TFIND & TRFD);
     eauto using match_callstack_match_globalenvs.
   monadInv TRFD.
   eexists _, _. intuition idtac.
   - econstructor; eauto.
   - econstructor; eauto.
-  - eapply match_callstack_match_globalenvs; eauto.
-  - inv H0. inv H. eexists. split.
+  - constructor; eauto using match_callstack_match_globalenvs.
+    + clear - MCS. induction MCS; cbn in *; eauto. destruct MENV. xomega.
+    + clear - MCS. induction MCS; cbn in *; eauto. destruct MENV. xomega.
+  - inv H1. inv H. eexists. split.
     + econstructor; eauto.
     + econstructor; eauto.
       apply match_callstack_incr_bound with (Mem.nextblock m) (Mem.nextblock tm).
@@ -2213,8 +2222,8 @@ Theorem transl_program_correct prog tprog:
 Proof.
   intros MATCH. split; [apply match_program_skel in MATCH; auto | ].
   intros w se1 se2 q1 q2 Hse1 SKEL Hse Hq.
-  split. { destruct Hq. eapply Genv.is_internal_transf_partial; eauto.
-           intros. destruct f; monadInv H3; cbn; auto. }
+  split. { destruct Hq, Hse. eapply Genv.is_internal_transf_partial; eauto.
+           intros. destruct f0; monadInv H6; cbn; auto. }
   eapply forward_simulation_star; eauto.
   apply transl_initial_states; eauto.
   apply transl_final_states; eauto.
